\documentclass[11pt]{article}
\usepackage[cm]{fullpage}
%%AVC PACKAGES
\usepackage{avcgreek}
\usepackage{avcfonts}
\usepackage{avcmath}
\usepackage[numberby=section]{avcthm}
\usepackage{qcmacros}
\usepackage{goldstone}
%%MACROS FOR THIS DOCUMENT
\numberwithin{equation}{section}
\usepackage[
  margin=1.5cm,
  includefoot,
  footskip=30pt,
  headsep=0.2cm,headheight=1.3cm
]{geometry}
\usepackage{fancyhdr}
\pagestyle{fancy}
\fancyhf{}
\fancyhead[LE,RO]{Quiz 7, Handout 1: Perturbative analysis}
\fancyfoot[CE,CO]{\thepage}
\usepackage{url}
\makeatother
\newcommand{\resolventline}[2][1]{
  \tikz[overlay]{
      \draw[thick,flexdotted] (0,-1ex) to ++(0,#1*4.5ex) node[above,inner sep=1pt] {#2};
  }
}

\newcommand{\fwkt}[1]{\kt{\makebox[0.8em][c]{\ensuremath{#1}}}}
\newcommand{\fwbr}[1]{\br{\makebox[0.8em][c]{\ensuremath{#1}}}}
\newcommand{\bord}[1]{\ensuremath{^{\scriptscriptstyle[#1]}}}

\begin{document}

\setlength{\abovedisplayskip}{3pt}
\setlength{\belowdisplayskip}{3pt}



\setcounter{section}{6}
\section{Perturbative analysis}

Now, just to be confusing, redefine some shit.
\begin{align}
  \bo{1}_\mr{i}
\equiv
\pma[l]{
  \bo{1} & \bo{0} \\
  \bo{0} & \bo{0}
}
&&
  \bo{1}_\mr{e}
\equiv
\pma[l]{
  \bo{0} & \bo{0} \\
  \bo{0} & \bo{1}
}
&&
  \bo{H}_\mr{xy}
\equiv
  \bo{1}_\mr{x}\,
  \bo{H}\,
  \bo{1}_\mr{y}
&&
  \bo{c}_\mr{x}
\equiv
  \bo{1}_\mr{x}\,
  \bo{c}
\end{align}

\begin{align}
  \bo{H}
=
  \bo{H}_\mr{ii}
+
  \bo{H}_\mr{ie}
+
  \bo{H}_\mr{ei}
+
  \bo{H}_\mr{ee}
\end{align}

\begin{align}
  \bo{R}_\mr{ee}
\equiv
\left.
  (
    E
  -
    \bo{H}
  )^{-1}
\right|_\mr{e}
&&
  \bo{R}_\mr{ee}
  (
    E
  -
    \bo{H}
  )
  \bo{1}_\mr{e}
=
  \bo{1}_\mr{e}
&&
\begin{array}{r@{\ }l}
  \bo{R}_\mr{ee}\,
  (
    E
  -
    \bo{H}
  )
&=
-
  \bo{R}_\mr{ee}\,
  \bo{H}_\mr{ei}
+
  \bo{1}_\mr{e}
\\
  (
    E
  -
    \bo{H}
  )\,
  \bo{R}_\mr{ee}
&=
-
  \bo{H}_\mr{ie}\,
  \bo{R}_\mr{ee}
+
  \bo{1}_\mr{e}
\end{array}
\end{align}
Operating the upper equation on $\bo{c}$ gives zero due to the Schr\"odinger equation, which implies
$
  \bo{c}_\mr{e}
=
  \bo{R}_\mr{ee}
  \bo{H}_\mr{ei}
  \bo{c}_\mr{i}
$.
Projecting the Schr\"odinger equation by $\bo{1}_\mr{i}$ and substituting in this result leads to the following.
\begin{align}
  (
    \bo{H}_\mr{ii}
  +
    \bo{V}_\mr{ii}
  )
  \bo{c}_\mr{i}
=
  E
  \bo{c}_\mr{i}
&&
  \bo{V}_\mr{ii}
\equiv
  \bo{H}_\mr{ie}
  \bo{R}_\mr{ee}
  \bo{H}_\mr{ei}
\end{align}

\begin{align}
  E
=
  \fr{
    \bo{c}_\mr{i}\dg
    (
      \bo{H}_\mr{ii}
    +
      \bo{V}_\mr{ii}
    )
    \bo{c}_\mr{i}
  }{
    \bo{c}_\mr{i}\cdot
    \bo{c}_\mr{i}
  }
\end{align}


\begin{align*}
  E
=
  \ip{\F|
  (
    1
  +
    \La
  )
  \ol{H}
  |\F}
+
  \ip{\F|\La\ol{H}|\bo{e}}
  \ip{\bo{e}|E - \ol{H}|\bo{e}}^{-1}
  \ip{\bo{e}|\ol{H}|\F}
\end{align*}

\begin{align*}
  \d E
=
  \ip{\F|\La\ol{H}|\bo{e}}
  \ip{\bo{e}|E - \ol{H}|\bo{e}}^{-1}
  \ip{\bo{e}|\ol{H}|\F}
\approx
  \ip{\F|\La\ol{H}\ord{1}|\bo{e}}
  \ip{\bo{e}|E\ord{0} - \ol{H}\ord{0}|\bo{e}}^{-1}
  \ip{\bo{e}|\ol{H}\ord{m}|\F}
\end{align*}


\begin{align}
  \ol{H}
=
  E_\mr{ref}
+
  H_0
+
  (
    H_0
    T
  +
    V_\mr{c}\,
    \mr{exp}(T)
  )_\mr{C}
\end{align}

\begin{align}
  \ol{H}\ord{0}
=
  E_\mr{ref}
+
  H_0
&&
  \ol{H}\ord{1}
=
  (H_0T\ord{1})_\mr{C}
+
  V_\mr{c}
&&
  \ol{H}\ord{2}
=
  (
    H_0
    T\ord{2}
  +
    V_\mr{c}\,
    T\ord{1}
  )_\mr{C}
\end{align}

\begin{align}
\end{align}

\newpage
\begin{align}
  \ol{H}
  \mc{R}_k
  \kt{\F}
=
  E_k
  \mc{R}_k
  \kt{\F}
&&
  \br{\F}
  \mc{L}_k
  \ol{H}
=
  \br{\F}
  \mc{L}_k
  \w_k
&&
  \fwbr{\F}
    \mc{L}_k
    \mc{R}_l
  {\F}
=
  \d_{kl}
&&
  \ol{H}
=
  \mr{exp}(-T)
  H\,
  \mr{exp}(T)
=
  E_\mr{ref}
+
  \ol{H}_\mr{c}
\end{align}
\textbf{Note to self:}
Go back and change $E_0$ to $E_\mr{ref}$ throughout to avoid problems like this ($E_0$ should refer to the ground state energy).\\
\textbf{Note to self:}
Go back and change $H_e$ to $H$ for simplicity.
\begin{align}
  \mc{R}_0
=
  1
&&
  \mc{L}_0
=
  1
+
  \La
&&
  \La
=
  \sum_{h=1}^n
  \La_h
&&
  \La_h
\equiv
  (\tfr{1}{h!})^2\,
  \la_{i_1\cd i_h}^{a_1\cd a_h}
  \tl{a}^{i_1\cd i_h}_{a_1\cd a_h}
\end{align}
\textbf{Note to self:}
Go back and change $k$ to $h$ for summations over excitation levels.
\begin{align*}
  E_\mr{c}
\equiv
  \fwbr{\F}\mc{L}_0\ol{H}\mc{R}_0{\F}
-
  E_\mr{ref}
=
  \fwbr{\F}(1+\La)\ol{H}_\mr{c}\fwkt{\F}
\end{align*}
Structure of matrix
\begin{align*}
  \ol{\bo{H}}_\mr{c}
=
\pma{
  E_\mr{c} & \fwbr{\F}\ol{H}_\mr{c}\fwkt{\bo{i}} & \fwbr{\F}\ol{H}_\mr{c}\fwkt{\bo{e}} \\
  \bo{0} & \fwbr{\bo{i}}\ol{H}_\mr{c}\fwkt{\bo{i}} & \fwbr{\bo{i}}\ol{H}_\mr{c}\fwkt{\bo{e}} \\
  \fwbr{\bo{e}}\ol{H}_\mr{c}\fwkt{\F} & \fwbr{\bo{e}}\ol{H}_\mr{c}\fwkt{\bo{i}} & \fwbr{\bo{e}}\ol{H}_\mr{c}\fwkt{\bo{e}} \\
}
&&
  \bo{i}
\equiv
\pma{
  \bo{s}_1 & \cd & \bo{s}_m
}
&&
  \bo{e}
\equiv
\pma{
  \bo{s}_{m-1} & \cd & \bo{s}_n
}
&&
  \bo{s}_h
\equiv
\pma{
  \cd
\
  \F_{i_1\cd i_h}^{a_1\hspace{-1pt}\cd a_h}
\
  \cd
}
\end{align*}


\begin{thm}
\thmtitle{Fa√† di Bruno's formula}
\begin{align}
  \pd{^n}{x_1\cd \pt x_n}
  f(g(\bm{x}))
=
  \sum_{k=1}^n
  \sum_{(\bm{x}_1,\ld,\bm{x}_k)}^{\mc{P}_k(\bm{x})}
  f\ord{k}(g(\bm{x}))
  \prod_{i=1}^k
  \pd{
    ^{|\bm{x}_i|}
    g(\bm{x})
  }{
    x_{i,1}
  \cd
    \pt
    x_{i,|\bm{x}_i|}
  }
\end{align}
\end{thm}


\end{document}