\documentclass[11pt]{article}
\usepackage[cm]{fullpage}
%%AVC PACKAGES
\usepackage{avcgreek}
\usepackage{avcfonts}
\usepackage{avcmath}
\usepackage[numberby=section,skip=9pt plus 2pt minus 7pt]{avcthm}
\usepackage{qcmacros}
\usepackage{goldstone}
%%MACROS FOR THIS DOCUMENT
\numberwithin{equation}{section}
\usepackage[
  margin=1.5cm,
  includefoot,
  footskip=30pt,
  headsep=0.2cm,headheight=1.3cm
]{geometry}
\usepackage{fancyhdr}
\pagestyle{fancy}
\fancyhf{}
\fancyhead[LE,RO]{Quiz 9, Handout 1: Response theory}
\fancyfoot[CE,CO]{\thepage}
\usepackage{url}
\makeatother
\newcommand{\resolventline}[2][1]{
  \tikz[overlay]{
      \draw[thick,flexdotted] (0,-1ex) to ++(0,#1*4.5ex) node[above,inner sep=1pt] {#2};
  }
}
\usepackage{accents}
\newcommand{\oc}[1]{\ensuremath{\accentset{\circ}{#1}}}
\newcommand{\wtl}[1]{\ensuremath{\widetilde{#1}}}

\begin{document}

\setlength{\abovedisplayskip}{5pt}
\setlength{\belowdisplayskip}{5pt}


\setcounter{section}{8}
\section{Response theory}


\newpage
\appendix

\section{Time-dependent perturbation theory}

\begin{rmk}
In an time-varying field, the electronic wavefunction is no longer simply an eigenfunction of the Hamiltonian.
This more general system is described by the following \textit{time-dependent Schr\"odinger equation}
\begin{align}
\label{eq:schrodinger-equation}
  H(t)
  \Y(t)
=
  i
  \pd{\Y(t)}{t}
&&
  H(t)
=
  H
+
  V(t)
\end{align}
where $H$ is the usual electronic Hamiltonian and $V(t)$ describes the interaction with the external field.
If the electrons are prepared in a particular state $\Y_0$ at some time $t_0$, the system is completely described by a \textit{time-evolution operator}.
\begin{align}
  \Y(t)=U(t,t_0)\Y_0
&&
  \Y_0
=
  \Y(t_0)
\end{align}
The following discussion shows how to expand this operator in orders of the perturbing interaction, $V(t)$.
\end{rmk}

\begin{dfn}
\thmtitle{Interaction picture}
The \textit{interaction picture} results from to the following similarity transformation.
\begin{align}
  \tl{\Th}(t)
\equiv
  e^{+iHt}
  \Th(t)
&&
  \tl{W}(t)
\equiv
  e^{+iHt}
  W(t)
  e^{-iHt}
\end{align}
Expanding the Schr\"odinger equation in the interaction picture yields the the \textit{Schwinger-Tomonaga equation}.
\begin{align}
\label{eq:schwinger-tomonaga}
  \tl{V}(t)
  \tl{\Y}(t)
=
  i
  \pd{\tl{\Y}(t)}{t}
\end{align}
Multiplying both sides by $-i$ and integrating from $t_0$ to $t$ yields a recursive equation for the interaction-picture wavefunction
\begin{align}
\label{eq:integrated-schwinger-tomonaga-equation}
  \tl{\Y}(t)
-
  \tl{\Y}(t_0)
=
-
  i
  \int_{t_0}^t
  dt'\,
  \tl{V}(t')
  \tl{\Y}(t')
\end{align}
from which we infer
$
  \tl{U}(t,t_0)
=
  1
-
  i
  \int_{t_0}^t
  dt'
  \tl{V}(t')\,
  \tl{U}(t',t_0)
$.
Infinite recursion of this identity leads to the following.
\begin{align}
  \tl{U}(t,t_0)
=
  \sum_{n=0}^\infty
  (-i)^n
  \int_{t_0}^t
  dt_1
  \int_{t_0}^{t_1}
  dt_2
  \cd
  \int_{t_0}^{t_{n-1}}
  dt_n
  \,
  \tl{V}(t_1)
  \cd
  \tl{V}(t_n)
\end{align}
\end{dfn}

\begin{dfn}
\thmtitle{Time-ordering}
Let 
$
  \tl{q}_1(t_1)\cd \tl{q}_n(t_n)
$
be a string of particle-hole operators in the interaction picture.\footnotemark
\footnotetext{
As in
$
  \tl{q}(t)
\equiv
  e^{+iHt}
  q
  e^{-iHt}
$
for some
$q\in\{a_p\}\cup\{a_p\dg\}$.
}
The \textit{time-ordering map} takes this string into
$
  \mc{T}\{
  \tl{q}_1(t_1)\cd \tl{q}_n(t_n)
  \}
\equiv
  \e_\pi \,\tl{q}_{\pi(1)}(t_{\pi(1)})\cd \tl{q}_{\pi(n)}(t_{\pi(n)})
$,
where $\pi\in\mr{S}_n$ is a permutation that puts the time arguments in reverse-chronological order, $t_{\pi(1)}>\cd>t_{\pi(n)}$.
\end{dfn}

\begin{ntt}
\begin{align}
  \int_{t_1,t_2,t_3,\ld}^{[t_0,t]}
  dt_1dt_2dt_3\cd
\equiv
  \int_{t_0}^t
  dt_1
  \int_{t_0}^t
  dt_2
  \int_{t_0}^t
  dt_3
  \cd
&&
  \int_{t_1>t_2>t_3>\cd}^{[t_0,t]}
  dt_1dt_2dt_3\cd
\equiv
  \int_{t_0}^t
  dt_1
  \int_{t_0}^{t_1}
  dt_2
  \int_{t_0}^{t_2}
  dt_3
  \cd
\end{align}
\begin{align}
  \int_{t_1\cd t_n}^{[t_0,t]}
  dt_1\cd t_n\,
  f(t_1\cd t_n)
=
  \sum_{\pi\in\mr{S}_n}
  \int_{t_{\pi(1)}>\ld>t_{\pi(n)}}^{[t_0,t]}
  dt_1\cd t_n\,
  f(t_1\cd t_n)
\end{align}
\end{ntt}


\begin{prop}
\thmtitle{The Dyson series}
\thmstatement{
$\ds{
  \tl{U}(t,t_0)
=
  \mc{T}\{
    e^{
    -
      i
      \int_{t_0}^t
      dt'\,
      \tl{V}(t')
    }
  \}
}$
}
\thmproof{
\begin{align}
  \sum_{n=0}^\infty
  \fr{(-i)^n}{n!}
  \int_{t_1\cd t_n}^{[t_0,t]}
  dt_1\cd dt_n\,
  \mc{T}\{
    \tl{V}(t_1)
    \cd
    \tl{V}(t_n)
  \}
=
  \sum_{n=0}^\infty
  \fr{(-i)^n}{n!}
  \sum_{\pi\in\mr{S}_n}
  \int_{t_{\pi(1)}>\ld>t_{\pi(n)}}^{[t_0,t]}
  dt_1\cd dt_n\,
  \mc{T}\{
    \tl{V}(t_1)
    \cd
    \tl{V}(t_n)
  \}
\end{align}
}
\end{prop}



\newpage
\section{Response functions}

\begin{rmk}
\begin{align}
  V(t)
=
  \sum_\b
  V_\b
  f_\b(t)
&&
  \lim_{t\rightarrow-\infty}
  f_\b(t)
=
  0
\end{align}
\begin{align}
  \tl{\Y}\ord{0}(t)
=
  \lim_{t\rightarrow-\infty}
  \tl{\Y}(t)
=
  \Y_0
&&
  H
  \Y_k
=
  E_k
  \Y_k
\end{align}
\begin{align}
  \tl{\Y}(t)
=
  \sum_{n=0}^\infty
  \tl{\Y}\ord{n}(t)
&&
  \tl{\Y}\ord{n}(t)
=
  \fr{(-i)^n}{n!}
  \int_{\mb{R}^n}
  dt_1\cd dt_n\,
  \th(t-t_1)
  \cd
  \th(t-t_n)\,
  \mc{T}\{
    \tl{V}(t_1)
    \cd
    \tl{V}(t_n)
  \}
  \Y_0
\end{align}
\end{rmk}

\begin{dfn}
\thmtitle{Response function}
\begin{align}
  X(t)
=
  \sum_{n=0}^\infty
  \fr{1}{n!}
  \sum_{\b_1,\ld,\b_n}
  \int_{\mb{R}^n}
  dt_1\cd t_n\,
  f_{\b_1}(t_1)
  \cd
  f_{\b_n}(t_n)\,
  X^{\b_1\cd \b_n}_{t;t_1\cd\,t_n}
&&
  X^{\b_1\cd \b_n}_{t;t_1\cd\,t_n}
\equiv
  \left.
  \fd{^n
    X(t)
  }{
    f_{\b_1}(t_1)
    \cd
    df_{\b_n}(t_n)
  }
  \right|_{\bm{f}=\bo{0}}
\end{align}
\end{dfn}

\begin{prop}
\begin{align}
  \Y^{\b_1\cd \b_n}_{t; t_1\cd t_n}
=
  (-i)^n
  \th(t-t_1)
  \cd
  \th(t-t_n)\,
  \mc{T}\{
    \tl{V}(t_1)
  \cd
    \tl{V}(t_n)
  \}
  \Y_0
\end{align}
\end{prop}

\begin{ntt}
\begin{align}
  \iip{\tl{W}(t); \tl{V}_{\b_1}(t_1),\ld,\tl{V}_{\b_n}(t_n)}
\equiv
  \left.
  \fd{^n
    \ip{\Y(t)|W(t)|\Y(t)}
  }{
    f_{\b_1}(t_1)
    \cd
    df_{\b_n}(t_n)
  }
  \right|_{\bm{f}=\bo{0}}
\end{align}
\end{ntt}

\begin{ex}
\begin{align}
  \tl{\Y}^{\b}_{t;t'}
=
  \left.
  \pd{\tl{\Y}(t)}{f_\b(t')}
  \right|_{\bm{f}=\bo{0}}
=
\end{align}
\end{ex}


\newpage
\section{Fourier transforms}


\begin{rmk}
\begin{align}
  f_\b(t)
=
  \int_{-\infty}^\infty
  d\w\,
  f_\b(\w)
  e^{-i\w t}
&&
  f_\b(\w)
\equiv
  (2\pi)^{-1}
  \int_{-\infty}^\infty
  dt\,
  f_\b(t)
  e^{+i\w t}
&&
  \w
\equiv
  \mr{Re}(\w)
+
  i\ev
\end{align}
$
  f_\b(-\w)
=
  f_\b^*(\w)
$\\
Footnote:
Fourier transforms can always be verified using
$\ds{
  \int_\mb{R}
  dk\,
  e^{ikx}
=
  2\pi\,\d(x)
}$
\end{rmk}


\begin{rmk}
Define $\ta_j\equiv t_j-t$
and note that
$
  X^{\b_1\cd \b_n}_{t;t_1\cd t_n}
=
  X^{\b_1\cd \b_n}_{0;\ta_1\cd \ta_n}
$
\begin{align}
  X^{\b_1\cd \b_n}_{0;\ta_1\cd \ta_n}
\equiv
  (2\pi)^{-n}
  \int_{\mb{R}^n}
  d\w_1\cd d\w_n\,
  X^{\b_1\cd \b_n}_{\w_1\cd\w_n}
  e^{+i\sum_j\w_j\ta_j}
&&
  X^{\b_1\cd \b_n}_{\w_1\cd\w_n}
\equiv
  \int_{\mb{R}^n}
  d\ta_1\cd d\ta_n\,
  X^{\b_1\cd \b_n}_{0;\ta_1\cd \ta_n}
  e^{-i\sum_j\w_j\ta_j}
\end{align}
\end{rmk}

\begin{rmk}
\thmstatement{
$\ds{
  \int_{\mb{R}^n}
  dt_1\cd dt_n\,
  f_{\b_1}(t_1)
  \cd
  f_{\b_n}(t_n)\,
  X_{t;t_1\cd t_n}^{\b_1\cd\b_n}
=
  \int_{\mb{R}^n}
  d\w_1\cd d\w_n\,
  f_{\b_1}(\w_1)
  \cd
  f_{\b_n}(\w_n)
  X^{\b_1\cd \b_n}_{\w_1\cd\w_n}
  e^{-i\sum_j\w_jt}
}$
}
\end{rmk}

\newpage
\section{Complex Calculus}


\end{document}